# Solutions to Apostol's Calculus Vol. 1

## I 3.3

### Theorem I.5

$$
\begin{align*}
a(b - c) &= a(b + (-c)) \\
&= ab + a(-c) \\
&= ab + a(-c) + (ac + (-(ac))) \\
&= ab + a(-c + c) + (-(ac)) \\
&= ab + a(0) + (-(ac)) \\
&= a(b + 0) + (-(ac)) \\
&= ab + (-(ac)) \\
&= ab - ac
\end{align*}
$$

### Theorem I.6

$$
\begin{align*}
0 \cdot a &= a \cdot 0 \\
&= a \cdot (a + (-a)) \\
&= a \cdot (a - a) \\
&= aa - aa \\
&= 0
\end{align*}
$$

### Theorem I.7

By Axiom 6, let $y$ be the real number such that $ay = 1$. Then,

$$
\begin{align*}
b &= (1)b \\
&= (ay)b \\
&= (ab)y \\
&= (ac)y \\
&= (ay)c \\
&= (1)c \\
&= c
\end{align*}
$$

### Theorem I.8

By Axiom 6, there exists $y \in \mathbb{R}$ such that $ay = 1$. Let $x = by$. Then,

$$
\begin{align*}
ax &= a(by) \\
&= b(ay) \\
&= b
\end{align*}
$$

Suppose that $\exists x_1, x_2 \in \mathbb{R}$ such that $ax_1 = ax_2 = b$. Then, by Theorem I.7, $x_1 = x_2$. Therefore, there is a unique $x$ such that $ax = b$.

### Theorem I.9

$$
\begin{align*}
b/a &= (aa^{-1})(b/a) \\
&= (a \cdot (b/a))(a^{-1}) \\
&= b \cdot a^{-1}
\end{align*}
$$

### Theorem I.10

$$
\begin{align*}
(a^{-1})^{-1} &= (aa^{-1})(a^{-1})^{-1} \\
&= a(a^{-1}(a^{-1})^{-1}) \\
&= a(1) \\
&= a
\end{align*}
$$

## Theorem I.11

WLOG, suppose $b \ne 0$. By Axiom 6 and Theorem I.8, $b^{-1}$ exists.

$$
\begin{align*}
ab = 0 &\implies a(b \cdot b^{-1}) = 0 \cdot b^{-1} \\
&\implies a(1) = 0 \\
&\implies a = 0
\end{align*}
$$

## Theorem I.12

$$
\begin{align*}
(-a)b &= ab + (-(ab)) + (-a)b \\
&= (a + (-a))b + (-(ab)) \\
&= (0)b + (-(ab)) \\
&= -(ab)
\end{align*}
$$

$$
\begin{align*}
(-a)(-b) &= -(a(-b)) \\
&= -((-b)a) \\
&= -(-(ba)) \\
&= -(-(ab)) \\
&= ab
\end{align*}
$$

